Keep proving the release operation of the semaphore

formal-proofs/theories/lib/interruptible_semaphore/interruptible_semaphore.v
@@ -33,6 +33,7 @@ Definition release_semaphore : val :=
 
 End impl.
 
+From iris.base_logic.lib Require Import invariants.
 From iris.heap_lang Require Import proofmode.
 From iris.algebra Require Import auth.
 From iris.algebra Require Import list gset excl csum.
@@ -43,7 +44,7 @@ Require Import SegmentQueue.lib.infinite_array.iterator.
 
 Section proof.
 
-Notation algebra := (authR (prodUR natUR natUR)).
+Notation algebra := (authR (prodUR (optionUR (exclR natO)) natUR)).
 
 Class semaphoreG Σ := SemaphoreG { semaphore_inG :> inG Σ algebra }.
 Definition semaphoreΣ : gFunctors := #[GFunctor algebra].
@@ -56,44 +57,64 @@ Notation iProp := (iProp Σ).
 
 Variable (segment_size: positive).
 
-Definition is_semaphore (R : iProp) (γ: gname) (availablePermits: nat) (p: loc)
+Definition is_semaphore_inv (R : iProp) (γ: gname) (availablePermits: nat) (p: loc)
   (epℓ eℓ dpℓ dℓ: loc) (γa γtq γe γd: gname) :=
   (∃ (readyToCancel: nat) l deqFront,
   ([∗ list] _ ∈ seq 0 availablePermits, R) ∗
-   own γ (● (availablePermits, readyToCancel)) ∗
-   is_thread_queue N segment_size True R γa γtq γe γd eℓ epℓ dℓ dpℓ l deqFront ∗
+   own γ (● (Excl' availablePermits, readyToCancel)) ∗
+   is_thread_queue (N .@ "tq") segment_size True R γa γtq γe γd eℓ epℓ dℓ dpℓ l deqFront ∗
    let v := count_matching still_present (drop deqFront l) in
    p ↦ #(availablePermits - v + readyToCancel) ∗
    ⌜readyToCancel <= v ∧ (availablePermits = 0 ∨ v = readyToCancel)%nat⌝)%I.
 
-Theorem release_semaphore_spec R γ (p epℓ eℓ dpℓ dℓ: loc) γa γtq γe γd:
-  R -∗
-  <<< ∀ availablePermits, is_semaphore R γ availablePermits p epℓ eℓ dpℓ dℓ γa γtq γe γd >>>
-    (release_semaphore segment_size) #p #dℓ #dpℓ @ ⊤
-  <<< is_semaphore R γ (1 + availablePermits)%nat p epℓ eℓ dpℓ dℓ γa γtq γe γd, RET #() >>>.
+Definition is_semaphore (R : iProp) (γ: gname) (p: loc)
+           (epℓ eℓ dpℓ dℓ: loc) (γa γtq γe γd: gname) :=
+  inv (N .@ "semaphore") (∃ availablePermits,
+            is_semaphore_inv R γ availablePermits p epℓ eℓ dpℓ dℓ γa γtq γe γd)%I.
+
+Definition semaphore_permits γ availablePermits :=
+  own γ (◯ (Excl' availablePermits, ε)).
+
+Theorem count_matching_find_index_Some A (P: A -> Prop) (H': forall x, Decision (P x)) l:
+  count_matching P l > 0 -> is_Some (find_index P l).
 Proof.
-  iIntros "HR" (Φ) "AU". wp_lam. wp_pures.
+  induction l; simpl; first done.
+  destruct (decide (P a)); first by eauto.
+  destruct (find_index P l); by eauto.
+Qed.
+
+Theorem release_semaphore_spec R γ (p epℓ eℓ dpℓ dℓ: loc) γa γtq γe γd:
+  is_semaphore R γ p epℓ eℓ dpℓ dℓ γa γtq γe γd -∗
+  R -∗
+  <<< ∀ availablePermits, semaphore_permits γ availablePermits >>>
+    (release_semaphore segment_size) #p #dpℓ #dℓ @ ⊤ ∖ ↑N
+  <<< semaphore_permits γ (1 + availablePermits)%nat, RET #() >>>.
+Proof.
+  iIntros "#HSemInv HR" (Φ) "AU". wp_lam. wp_pures.
   wp_bind (FAA _ _).
-  iMod "AU" as (availablePermits) "[HIsSem HClose]".
-  iDestruct "HIsSem" as (readyToCancel l deqFront) "(HPerms & HAuth & HTq & Hp & HPure)".
+  iInv "HSemInv" as (availablePermits' readyToCancel l deqFront)
+                      "(HPerms & >HAuth & HTq & Hp & >HPure)" "HInvClose".
   iDestruct "HPure" as %HPure.
   remember (count_matching _ _) as v.
-  remember (availablePermits - v + readyToCancel) as op.
+  remember (availablePermits' - v + readyToCancel) as op.
   wp_faa.
   destruct (decide (0 <= op)).
   {
-    iDestruct "HClose" as "[_ HClose]".
-    iMod (own_update with "HAuth") as "[HAuth HFrag]".
+    iMod "AU" as (availablePermits) "[HFrag HCloseAU]".
+    iDestruct (own_valid_2 with "HAuth HFrag") as
+        %[[<-%Excl_included%leibniz_equiv _]%prod_included _]%auth_both_valid.
+    iMod (own_update_2 with "HAuth HFrag") as "[HAuth HFrag]".
     {
-      apply auth_update_alloc.
-      apply prod_local_update_1.
-      apply (nat_local_update availablePermits 0%nat _ 1%nat).
-      auto.
+      apply auth_update, prod_local_update_1, option_local_update.
+      apply (exclusive_local_update _ (Excl (1 + availablePermits)%nat)).
+      done.
     }
     repeat rewrite Nat.add_1_r.
-    iMod ("HClose" with "[-]") as "HΦ".
+    iMod ("HCloseAU" with "HFrag") as "HΦ".
+    iMod ("HInvClose" with "[-HΦ]") as "_".
     {
-      iExists _, _, _. simpl. iFrame "HR HAuth HTq".
+      iExists _, _, _, _. simpl. iFrame "HAuth HTq". simpl.
+      iFrame "HR".
       iSplitL "HPerms".
       {
         iApply (big_opL_forall' with "HPerms").
@@ -116,19 +137,76 @@ Proof.
   }
 
   assert (v > 0) as HExistsNondequed by lia.
-  move: HExistsNondequed. subst; clear. move=> HExistsNondequed.
+  move: HExistsNondequed. subst. move=> HExistsNondequed.
 
-  iDestruct "HTq" as "(HInfArr & HListContents & HRest)".
+  apply count_matching_find_index_Some in HExistsNondequed.
+  destruct HExistsNondequed as [? HFindIndex].
+
+  iDestruct "HTq" as "(HInfArr & HListContents & HCancA & % & HRest)".
   iDestruct (cell_list_contents_register_for_dequeue
-               with "HR HListContents") as ">[[HAwak HDeqFront] [HListContents _]]".
+               with "HR HListContents") as ">[[HAwak #HDeqFront] [HListContents HCounts]]".
+  by eauto.
+  iDestruct "HCounts" as %HCounts.
+
+  iMod ("HInvClose" with "[-HAwak AU]") as "_".
   {
-    admit.
+    iExists _, _, _, _. iFrame "HListContents". iFrame.
+    iSplitL "HRest".
+    {
+      iDestruct "HRest" as (enqIdx deqIdx) "(HIt1 & HIt2 & HAwaks & HSusps & %)".
+      apply find_index_Some in HFindIndex.
+      destruct HFindIndex as [[? [HC HPres]] HNotPres].
+      rewrite lookup_drop in HC.
+      iSplitR.
+      {
+        iPureIntro.
+        intros [_ (? & ? & HOk)].
+        replace (deqFront + S x - 1)%nat with (deqFront + x)%nat in HOk by lia.
+        by simplify_eq.
+      }
+      iExists _, _. iFrame.
+      iPureIntro.
+      repeat split; try lia.
+      assert (deqFront + x < length l)%nat; try lia.
+      apply lookup_lt_is_Some. by eauto.
+    }
+    iSplitL.
+    {
+      rewrite HCounts.
+      clear.
+      remember (count_matching _ _) as v.
+      replace (availablePermits' - S v + readyToCancel + 1)
+              with (availablePermits' - v + readyToCancel) by lia.
+      done.
+    }
+    iPureIntro.
+    lia.
   }
 
-  iDestruct "HClose" as "[HClose _]".
-  iMod ("HClose" with "[-HDeqFront HAwak]") as "HΦ".
+  iModIntro. wp_pures. rewrite bool_decide_decide.
+  rewrite decide_False; auto.
+  wp_pures. wp_lam. wp_pures.
+
+  awp_apply (try_deque_thread_spec (N .@ "tq") with "HAwak").
+  iInv "HSemInv" as (? ? ? ?) "(HPerms & >HAuth & HTq & HRest)".
+  iApply (aacc_aupd with "AU"); first by solve_ndisj.
+  iIntros (availablePermits) "HPerms'".
+  iAaccIntro with "HTq".
   {
-    iExists _, _, _. iFrame "HAuth HPerms HInfArr".
+    iFrame "HPerms'".
+    iIntros "HTq !> $ !>".
+    iExists _, _, _, _. iFrame.
+  }
+  iIntros (?) "[_ HState]".
+  iDestruct "HState" as (i) "[HState|HState]".
+  {
+    iRight.
+    iDestruct "HState" as "[(% & -> & HTq) HRend]".
+    iMod (own_update_2 with "HAuth HPerms'") as "[HAuth HPerms']".
+    apply auth_update.
+    2: iFrame "HPerms'".
+    {
+      apply prod_local_update_1, option_local_update.
 
 Abort.
 
